compiler/src/examples/TestFlatImp.v
@@ -61,6 +61,7 @@ Existing Instance annoying_eq.
 Instance myFlatImpParams: FlatImp.parameters := {|
   FlatImp.Event := Empty_set;
   FlatImp.ext_spec action t args outcome := False;
+  FlatImp.max_ext_call_code_size name := 0%Z;
 |}.
 
 Definition eval_stmt_test fuel initialSt := eval_stmt empty_map fuel initialSt no_mem.
